Drop explicit persistence --- trivial fixes (doesn't compile)
Compilation is restored by the next commits. This one should contain boring
changes.

This commit also undoes the changes to hkdot in the previous one, and fixes
things properly.

theories/Dot/examples/sem/semtyp_lemmas/sub_lr.v
@@ -16,7 +16,7 @@ Section defs.
 
   (** Legacy: (double)-indexed subtyping. *)
   Definition sstpi `{!dlangG Σ} i j Γ τ1 τ2 : iProp Σ :=
-    □∀ ρ v,
+    ∀ ρ v,
       sG⟦Γ⟧*ρ → ▷^i oClose τ1 ρ v → ▷^j oClose τ2 ρ v.
   Global Arguments sstpi /.
 
@@ -54,7 +54,7 @@ Section judgment_lemmas.
   (** ** Show this typing judgment is equivalent to the more direct definition. *)
   Lemma istpi_eq Γ T1 i T2 j :
     Γ ⊨ T1, i <: T2, j ⊣⊢
-    □∀ ρ v, G⟦Γ⟧ ρ → ▷^i V⟦T1⟧ vnil ρ v → ▷^j V⟦T2⟧ vnil ρ v.
+    ∀ ρ v, G⟦Γ⟧ ρ → ▷^i V⟦T1⟧ vnil ρ v → ▷^j V⟦T2⟧ vnil ρ v.
   Proof. reflexivity. Qed.
 
   Lemma sstpi_app ρ Γ T1 T2 i j :
@@ -82,27 +82,27 @@ Section StpLemmas.
   Context `{HdotG: !dlangG Σ}.
 
   Lemma sSub_Refl {Γ} T i : ⊢ Γ s⊨ T, i <: T, i.
-  Proof. by iIntros "!> **". Qed.
+  Proof. by iIntros "/= **". Qed.
 
   Lemma sSub_Trans {Γ T1 T2 T3 i1 i2 i3} :
     Γ s⊨ T1, i1 <: T2, i2 -∗ Γ s⊨ T2, i2 <: T3, i3 -∗ Γ s⊨ T1, i1 <: T3, i3.
   Proof.
-    iIntros "#Hsub1 #Hsub2 !> * #Hg HT".
+    iIntros "#Hsub1 #Hsub2 %ρ * #Hg HT".
     iApply ("Hsub2" with "Hg (Hsub1 Hg HT)").
   Qed.
 
   Lemma sSub_Top Γ T i:
     ⊢ Γ s⊨ T, i <: oTop, i.
-  Proof. by iIntros "!> ** /=". Qed.
+  Proof. by iIntros "/= **". Qed.
 
   Lemma sBot_Sub Γ T i:
     ⊢ Γ s⊨ oBot, i <: T, i.
-  Proof. by iIntros "/= !> ** !>". Qed.
+  Proof. by iIntros "/= ** !>". Qed.
 
   Lemma sAnd1_Sub Γ T1 T2 i: ⊢ Γ s⊨ oAnd T1 T2, i <: T1, i.
-  Proof. by iIntros "/= !> * ? [? ?]". Qed.
+  Proof. by iIntros "/= * ? [? ?]". Qed.
   Lemma sAnd2_Sub Γ T1 T2 i: ⊢ Γ s⊨ oAnd T1 T2, i <: T2, i.
-  Proof. by iIntros "/= !> * ? [? ?]". Qed.
+  Proof. by iIntros "/= * ? [? ?]". Qed.
 
   Lemma sSub_And Γ T U1 U2 i j:
     Γ s⊨ T, i <: U1, j -∗
@@ -111,9 +111,9 @@ Section StpLemmas.
   Proof. rewrite !sstpi_to_sstpd0 sTEq_oAnd_oLaterN. apply sStp_And. Qed.
 
   Lemma sSub_Or1 Γ T1 T2 i: ⊢ Γ s⊨ T1, i <: oOr T1 T2, i.
-  Proof. by iIntros "!> * _ ? !> /="; eauto. Qed.
+  Proof. by iIntros "/= * _ ? !> /="; eauto. Qed.
   Lemma sSub_Or2 Γ T1 T2 i: ⊢ Γ s⊨ T2, i <: oOr T1 T2, i.
-  Proof. by iIntros "!> * _ ? !> /="; eauto. Qed.
+  Proof. by iIntros "/= * _ ? !> /="; eauto. Qed.
 
   Lemma sOr_Sub Γ T1 T2 U i j:
     Γ s⊨ T1, i <: U, j -∗
@@ -123,26 +123,26 @@ Section StpLemmas.
 
   Lemma sDistr_And_Or_Sub {Γ S T U i}:
     ⊢ Γ s⊨ oAnd (oOr S T) U , i <: oOr (oAnd S U) (oAnd T U), i.
-  Proof. iIntros "!> %% #Hg [[HS|HT] Hu] !> /="; [iLeft|iRight]; iFrame. Qed.
+  Proof. iIntros "%% #Hg [[HS|HT] Hu] !> /="; [iLeft|iRight]; iFrame. Qed.
 
   Lemma sSub_Add_Later Γ T i :
     ⊢ Γ s⊨ T, i <: oLater T, i.
-  Proof. by iIntros "!> ** !> /=". Qed.
+  Proof. by iIntros "/= ** !>". Qed.
 
   Lemma sLater_Sub Γ T i :
     ⊢ Γ s⊨ oLater T, i <: T, i.+1.
-  Proof. by iIntros "/= !> %ρ %v #HG #HT !>". Qed.
+  Proof. by iIntros "/= %ρ %v #HG #HT !>". Qed.
 
   Lemma sSub_Later Γ T i :
     ⊢ Γ s⊨ T, i.+1 <: oLater T, i.
-  Proof. by iIntros "/= !> ** !>". Qed.
+  Proof. by iIntros "/= ** !>". Qed.
 
   (** ** Subtyping for type selections. *)
   Lemma sSub_Sel {Γ L U p l i}:
     Γ s⊨p p : cTMem l L U, i -∗
     Γ s⊨ L, i <: oSel p l, i.
   Proof.
-    iIntros "/= #Hp !> %ρ %v Hg #HL"; iSpecialize ("Hp" with "Hg"); iNext i.
+    iIntros "/= #Hp %ρ %v Hg #HL"; iSpecialize ("Hp" with "Hg"); iNext i.
     iApply (path_wp_wand with "Hp"); iIntros (w).
     iApply (vl_sel_lb with "HL").
   Qed.
@@ -151,7 +151,7 @@ Section StpLemmas.
     Γ s⊨p p : cTMem l L U, i -∗
     Γ s⊨ oSel p l, i <: U, i.
   Proof.
-    iIntros "#Hp !> %ρ %v Hg Hφ"; iSpecialize ("Hp" with "Hg"); iNext i.
+    iIntros "#Hp %ρ %v Hg Hφ"; iSpecialize ("Hp" with "Hg"); iNext i.
     iDestruct (path_wp_agree with "Hp Hφ") as (w Hw) "[Hp Hφ]".
     iApply (vl_sel_ub with "Hφ Hp").
   Qed.
@@ -165,7 +165,7 @@ Section StpLemmas.
     oLaterN i T1 :: Γ s⊨ T1, i <: T2, j -∗
     Γ s⊨ oMu T1, i <: oMu T2, j.
   Proof.
-    iIntros "/= #Hstp !> %ρ %v #Hg #HT1".
+    iIntros "/= #Hstp %ρ %v #Hg #HT1".
     iApply ("Hstp" $! (v .: ρ) v with "[$Hg $HT1] [$HT1]").
   Qed.
 
@@ -186,7 +186,7 @@ Section StpLemmas.
   (** Novel subtyping rules. [Sub_Bind_1] and [Sub_Bind_2] become
   derivable. *)
   Lemma sMu_Sub {Γ T i} : ⊢ Γ s⊨ oMu (shift T), i <: T, i.
-  Proof. iIntros "!> **". by rewrite oMu_shift. Qed.
+  Proof. iIntros "%ρ **". by rewrite oMu_shift. Qed.
 
   Lemma Mu_Sub {Γ} T i: ⊢ Γ ⊨ TMu (shift T), i <: T, i.
   Proof.
@@ -196,7 +196,7 @@ Section StpLemmas.
   Qed.
 
   Lemma sSub_Mu {Γ T i} : ⊢ Γ s⊨ T, i <: oMu (shift T), i.
-  Proof. iIntros "!> **". by rewrite oMu_shift. Qed.
+  Proof. iIntros "%ρ **". by rewrite oMu_shift. Qed.
 
   Lemma Sub_Mu {Γ} T i: ⊢ Γ ⊨ T, i <: TMu (shift T), i.
   Proof.
@@ -210,7 +210,7 @@ Section StpLemmas.
     Γ s⊨ T1, i <: T2, i -∗
     Γ s⊨ cVMem l T1, i <: cVMem l T2, i.
   Proof.
-    iIntros "#Hsub !> %ρ %v Hg HT1"; iApply (cVMem_respects_subN with "[Hg] HT1").
+    iIntros "#Hsub %ρ %v Hg HT1"; iApply (cVMem_respects_subN with "[Hg] HT1").
     iApply (sstpi_app with "Hsub Hg").
   Qed.
 
@@ -262,7 +262,7 @@ Section StpLemmas.
     Γ s⊨p p : T, i -∗
     Γ s⊨ oSing p, i <: T, i.
   Proof.
-    iIntros "#Hp !> %ρ %v Hg /= Heq"; iSpecialize ("Hp" with "Hg"); iNext i.
+    iIntros "#Hp %ρ %v Hg /= Heq"; iSpecialize ("Hp" with "Hg"); iNext i.
     iDestruct "Heq" as %->%(alias_paths_elim_eq (T _ ρ)).
     by rewrite path_wp_pv_eq.
   Qed.
@@ -272,7 +272,7 @@ Section StpLemmas.
     Γ s⊨ oSing p, i <: oSing q, i -∗
     Γ s⊨ oSing q, i <: oSing p, i.
   Proof.
-    iIntros "#Hp #Hps !> %ρ %v #Hg Heq".
+    iIntros "#Hp #Hps %ρ %v #Hg Heq".
     iDestruct (path_wp_eq with "(Hp Hg)") as (w) "[Hpw _] {Hp}".
     rewrite -alias_paths_pv_eq_1; iSpecialize ("Hps" $! _ w with "Hg Hpw");
       iNext i; rewrite /= !alias_paths_pv_eq_1.
@@ -286,7 +286,7 @@ Section StpLemmas.
     Γ s⊨p p : oSing q, i -∗
     Γ s⊨ T1, i <: T2, i.
   Proof.
-    iIntros "#Hrepl #Hal !> %ρ %v Hg HT1".
+    iIntros "#Hrepl #Hal %ρ %v Hg HT1".
     iSpecialize ("Hal" with "Hg"); iNext i.
     iDestruct "Hal" as %Hal%alias_paths_simpl.
     iRewrite -("Hrepl" $! vnil ρ v Hal); iExact "HT1".
@@ -306,7 +306,7 @@ Section StpLemmas.
     (*───────────────────────────────*)
     Γ s⊨p p : T2, i + j.
   Proof.
-    iIntros "/= * #HpT1 #Hsub !> * #Hg".
+    iIntros "/= * #HpT1 #Hsub * #Hg".
     iSpecialize ("HpT1" with "Hg").
     rewrite !path_wp_eq.
     iDestruct "HpT1" as (v) "Hpv"; iExists v.
@@ -337,13 +337,13 @@ Section VarianceStpLemmas.
   Lemma sAnd_All_Sub_Distr Γ T U1 U2 i:
     ⊢ Γ s⊨ oAnd (oAll T U1) (oAll T U2), i <: oAll T (oAnd U1 U2), i.
   Proof.
-    iIntros "/= !> %ρ %v #Hg [#H1 #H2]". iNext.
+    iIntros "/= %ρ %v #Hg [#H1 #H2]". iNext.
     iDestruct "H1" as (t ?) "#H1"; iDestruct "H2" as (t' ->) "#H2"; simplify_eq.
     iExists _; iSplit => //.
-    iIntros "!>" (w) "#HT".
+    iIntros (w) "#HT".
     iSpecialize ("H1" with "HT").
     iSpecialize ("H2" with "HT").
-    iNext. iModIntro.
+    iNext.
     (* Oh. Dreaded conjunction rule. Tho could we use a version
     for separating conjunction? *)
     iApply wp_and. by iApply "H1". by iApply "H2".
@@ -352,7 +352,7 @@ Section VarianceStpLemmas.
   Lemma sAnd_Fld_Sub_Distr Γ l T1 T2 i:
     ⊢ Γ s⊨ oAnd (cVMem l T1) (cVMem l T2), i <: cVMem l (oAnd T1 T2), i.
   Proof.
-    iIntros "/= !> %ρ %v #Hg [#H1 H2]". iNext.
+    iIntros "/= %ρ %v #Hg [#H1 H2]". iNext.
     iDestruct "H1" as (d? pmem?) "#H1"; iDestruct "H2" as (d'? pmem'?) "#H2". objLookupDet.
     repeat (iExists _; repeat iSplit => //).
     by iApply (path_wp_and' with "H1 H2").
@@ -361,13 +361,12 @@ Section VarianceStpLemmas.
   Lemma sAnd_Typ_Sub_Distr Γ l L U1 U2 i:
     ⊢ Γ s⊨ oAnd (cTMem l L U1) (cTMem l L U2), i <: cTMem l L (oAnd U1 U2), i.
   Proof.
-    iIntros "/= !> %ρ %v Hg [H1 H2]". iNext.
+    iIntros "/= %ρ %v Hg [H1 H2]". iNext.
     iDestruct "H1" as (d? φ) "#[Hsφ1 [#HLφ1 #HφU1]]"; iDestruct "H2" as (d'? φ') "#[Hsφ2 [_ #HφU2]]".
     objLookupDet.
     iExists d; repeat iSplit => //.
     iExists φ; repeat iSplit => //.
-    iModIntro; iSplit; iIntros (w) "Hw".
-    - by iApply "HLφ1".
+    iIntros (w) "Hw".
     - iDestruct (dm_to_type_agree vnil w with "Hsφ1 Hsφ2") as "#Hag {Hsφ1 Hsφ2 HLφ1}".
       iSplit; [iApply "HφU1" | iApply "HφU2"] => //.
       iNext. by iRewrite -"Hag".
