theories/Dot/semtyp_lemmas/path_repl_lr.v
@@ -21,7 +21,7 @@ Section semantic_lemmas.
     Γ s⊨p p : τ, i -∗
     Γ s⊨p p : oSing p, i.
   Proof.
-    iIntros "#Hep !> %ρ Hg"; iApply (strong_path_wp_wand with "(Hep Hg)").
+    iIntros "#Hep %ρ Hg"; iApply (strong_path_wp_wand with "(Hep Hg)").
     iIntros "%v %Hpv _ !%"; apply alias_paths_pv_eq_1, Hpv.
   Qed.
 
@@ -29,7 +29,7 @@ Section semantic_lemmas.
     Γ s⊨p p : T, i -∗
     Γ s⊨ oSing p <:[i] T.
   Proof.
-    rewrite sstpd_eq; iIntros "#Hp !> %ρ %v Hg".
+    rewrite sstpd_eq; iIntros "#Hp %ρ %v Hg".
     iSpecialize ("Hp" with "Hg"); iNext i.
     iDestruct 1 as %->%(alias_paths_elim_eq (T _ ρ)).
     by rewrite path_wp_pv_eq.
@@ -40,7 +40,7 @@ Section semantic_lemmas.
     Γ s⊨ oSing p <:[i] oSing q -∗
     Γ s⊨ oSing q <:[i] oSing p.
   Proof.
-    rewrite !sstpd_eq; iIntros "#Hp #Hps !> %ρ %v #Hg".
+    rewrite !sstpd_eq; iIntros "#Hp #Hps %ρ %v #Hg".
     iDestruct (path_wp_eq with "(Hp Hg)") as (w) "[Hpw _] {Hp}".
     rewrite -alias_paths_pv_eq_1; iSpecialize ("Hps" $! _ w with "Hg Hpw");
       iNext i; rewrite /= !alias_paths_pv_eq_1.
@@ -52,7 +52,7 @@ Section semantic_lemmas.
     Γ s⊨p p : oSing q, i -∗
     Γ s⊨p q : oTop, i.
   Proof.
-    iIntros "#Hpq !> %ρ Hg /="; iSpecialize ("Hpq" with "Hg"); iNext i.
+    iIntros "#Hpq %ρ Hg /="; iSpecialize ("Hpq" with "Hg"); iNext i.
     iDestruct "Hpq" as %(v & _ & Hqv)%alias_paths_simpl%alias_paths_sameres.
     iIntros "!%". exact: (path_wp_pure_wand Hqv).
   Qed.
@@ -64,7 +64,7 @@ Section semantic_lemmas.
     Γ s⊨p p : oSing q, i -∗
     Γ s⊨ T1 <:[i] T2.
   Proof.
-    rewrite sstpd_eq; iIntros "#Hrepl #Hal !> %ρ %v #Hg".
+    rewrite sstpd_eq; iIntros "#Hrepl #Hal %ρ %v #Hg".
     iSpecialize ("Hal" with "Hg"); iNext i.
     iDestruct "Hal" as %Hal%alias_paths_simpl.
     iRewrite ("Hrepl" $! vnil ρ v Hal); iIntros "$".
@@ -81,7 +81,7 @@ Section semantic_lemmas.
   Lemma sP_Mu_E {Γ T p i} :
     Γ s⊨p p : oMu T, i -∗ Γ s⊨p p : T .sTp[ p /], i.
   Proof.
-    iIntros "#Hp !> %ρ Hg /=".
+    iIntros "#Hp %ρ Hg /=".
     iApply (strong_path_wp_wand with "(Hp Hg)"); iIntros "**".
     by rewrite oMu_eq sem_psubst_one_repl ?alias_paths_pv_eq_1.
   Qed.
@@ -89,7 +89,7 @@ Section semantic_lemmas.
   Lemma sP_Mu_I {Γ T p i} :
     Γ s⊨p p : T .sTp[ p /], i -∗ Γ s⊨p p : oMu T, i.
   Proof.
-    iIntros "#Hp !> %ρ Hg /=".
+    iIntros "#Hp %ρ Hg /=".
     iApply (strong_path_wp_wand with "(Hp Hg)"); iIntros "**".
     by rewrite oMu_eq sem_psubst_one_repl ?alias_paths_pv_eq_1.
   Qed.
@@ -100,7 +100,7 @@ Section semantic_lemmas.
   Lemma P_Mu_E {Γ T T' p i} (Hrepl : T .Tp[ p /]~ T') :
     Γ ⊨p p : TMu T, i -∗ Γ ⊨p p : T', i.
   Proof.
-    rewrite /iptp sP_Mu_E; iIntros "#Hp !> %ρ Hg /=".
+    rewrite /iptp sP_Mu_E; iIntros "#Hp %ρ Hg /=".
     iApply (strong_path_wp_wand with "(Hp Hg)"); iIntros "**".
     by rewrite (sem_psubst_one_eq Hrepl) ?alias_paths_pv_eq_1.
   Qed.
@@ -108,7 +108,7 @@ Section semantic_lemmas.
   Lemma P_Mu_I {Γ T T' p i} (Hrepl : T .Tp[ p /]~ T') :
     Γ ⊨p p : T', i -∗ Γ ⊨p p : TMu T, i.
   Proof.
-    rewrite /iptp -sP_Mu_I; iIntros "#Hp !> %ρ Hg /=".
+    rewrite /iptp -sP_Mu_I; iIntros "#Hp %ρ Hg /=".
     iApply (strong_path_wp_wand with "(Hp Hg)"); iIntros "**".
     by rewrite (sem_psubst_one_eq Hrepl) ?alias_paths_pv_eq_1.
   Qed.
@@ -118,7 +118,7 @@ Section semantic_lemmas.
   Lemma P_Mu_E' {Γ T T' p i} (Hrepl : T .Tp[ p /]~ T') :
     Γ ⊨p p : TMu T, i -∗ Γ ⊨p p : T', i.
   Proof.
-    iIntros "#Hp !> %ρ Hg /=".
+    iIntros "#Hp %ρ Hg /=".
     iApply (strong_path_wp_wand with "(Hp Hg)"); iIntros "**".
     by rewrite oMu_eq -(psubst_one_repl Hrepl) ?alias_paths_pv_eq_1.
   Qed.
@@ -126,7 +126,7 @@ Section semantic_lemmas.
   Lemma P_Mu_I' {Γ T T' p i} (Hrepl : T .Tp[ p /]~ T') :
     Γ ⊨p p : T', i -∗ Γ ⊨p p : TMu T, i.
   Proof.
-    iIntros "#Hp !> %ρ Hg /=".
+    iIntros "#Hp %ρ Hg /=".
     iApply (strong_path_wp_wand with "(Hp Hg)"); iIntros "**".
     by rewrite oMu_eq -(psubst_one_repl Hrepl) ?alias_paths_pv_eq_1.
   Qed.
@@ -137,7 +137,7 @@ Section semantic_lemmas.
     (*────────────────────────────────────────────────────────────*)
     Γ s⊨ tapp e1 (path2tm p2) : T2 .sTp[ p2 /].
   Proof.
-    iIntros "#He1 #Hp2 !> %ρ #Hg !>"; iSpecialize ("Hp2" with "Hg").
+    iIntros "#He1 #Hp2 %ρ #Hg"; iSpecialize ("Hp2" with "Hg").
     smart_wp_bind (AppLCtx _) v "Hr {He1}" ("He1" with "Hg").
     iDestruct "Hr" as (t ->) "#HvFun {Hg}"; rewrite path_wp_eq path2tm_subst.
     iDestruct "Hp2" as (pw Hpwpp) "Hpw"; iSpecialize ("HvFun" with "Hpw").
@@ -154,7 +154,7 @@ Section semantic_lemmas.
     (*────────────────────────────────────────────────────────────*)
     Γ ⊨ tapp e1 (path2tm p2) : T2'.
   Proof.
-    iIntros "#He1 #Hp2 !> * #Hg !>".
+    iIntros "#He1 #Hp2 %ρ #Hg".
     iDestruct (path_wp_eq with "(Hp2 Hg)") as (pw Hal%alias_paths_pv_eq_1) "_".
     iDestruct (sT_All_E_p with "He1 Hp2") as "{He1 Hp2} Hep".
     iApply (wp_wand with "(Hep Hg)"); iIntros "{Hep Hg} * #Hv".
@@ -167,7 +167,7 @@ Section semantic_lemmas.
     (*─────────────────────────*)
     Γ s⊨p p : cVMem l T, i.
   Proof.
-    iIntros "#HE /= !> %ρ Hg"; iSpecialize ("HE" with "Hg"); iNext i.
+    iIntros "#HE /= %ρ Hg"; iSpecialize ("HE" with "Hg"); iNext i.
     rewrite path_wp_pself_eq; iDestruct "HE" as (v q Hlook) "[Hpv #Htw]".
     iApply (path_wp_wand with "Hpv"). iIntros "/= % <-"; eauto.
   Qed.
@@ -175,7 +175,7 @@ Section semantic_lemmas.
   (* Suppose path typing required termination *now* rather than later:
 
     Definition sptp `{!dlangG Σ} p i Γ (T : oltyO Σ 0): iProp Σ :=
-     □∀ ρ, sG⟦Γ⟧* ρ →
+     ∀ ρ, sG⟦Γ⟧* ρ →
 -      ▷^i path_wp p.|[ρ] (λ v, oClose T ρ v).
 +      path_wp p.|[ρ] (λ v, ▷^i oClose T ρ v).
 
@@ -187,7 +187,7 @@ Section semantic_lemmas.
     (*─────────────────────────*)
     Γ s⊨p pself p l : T, i.
   Proof.
-    iIntros "#HE !> %ρ HG /="; iSpecialize ("HE" with "HG"); iNext i.
+    iIntros "#HE %ρ Hg /="; iSpecialize ("HE" with "Hg"); iNext i.
     rewrite path_wp_pself_eq path_wp_eq.
     iDestruct "HE" as (vp Hpv d Hlook pmem ->) "#H".
     iExists vp, pmem. eauto.
@@ -200,7 +200,7 @@ Section semantic_lemmas.
     Γ s⊨p q : T, i -∗
     Γ s⊨p p : T, i.
   Proof.
-    iIntros "#Hep #Heq !> %ρ #Hg"; iSpecialize ("Heq" with "Hg").
+    iIntros "#Hep #Heq %ρ #Hg"; iSpecialize ("Heq" with "Hg").
     iSpecialize ("Hep" with "Hg"); iNext i.
     by iDestruct "Hep" as %->%alias_paths_simpl%(alias_paths_elim_eq (T _ _)).
   Qed.
@@ -210,7 +210,7 @@ Section semantic_lemmas.
     Γ s⊨p pself q l : τ, i -∗
     Γ s⊨p pself p l : oSing (pself q l), i.
   Proof.
-    iIntros "#Hpq #HqlT !> %ρ #Hg"; iSpecialize ("HqlT" with "Hg");
+    iIntros "#Hpq #HqlT %ρ #Hg"; iSpecialize ("HqlT" with "Hg");
     iSpecialize ("Hpq" with "Hg"); iNext i; iClear "Hg".
     iDestruct "Hpq" as %Hal%alias_paths_simpl.
     rewrite !path_wp_eq; iDestruct "HqlT" as (vql Hql) "_".
@@ -224,7 +224,7 @@ Section semantic_lemmas.
     (*───────────────────────────────*)
     Γ s⊨p p : T2, i.
   Proof.
-    iIntros "#HpT1 #Hsub !> %ρ #Hg".
+    iIntros "#HpT1 #Hsub %ρ #Hg".
     iSpecialize ("Hsub" with "Hg"); iSpecialize ("HpT1" with "Hg"); iNext i.
     iApply (path_wp_wand with "HpT1"); iIntros "%w HvT1 {Hg HpT1}".
     iApply ("Hsub" with "HvT1").
