theories/Dot/semtyp_lemmas/prims_lr.v
@@ -50,13 +50,13 @@ Section Sec.
   Import path_wp.
   Lemma sP_Nat_I Γ n: ⊢ Γ s⊨p pv (vint n): oInt, 0.
   Proof.
-    iIntros "!> * _ /=";
+    iIntros "%ρ * _ /=";
       rewrite path_wp_pv_eq /= /pure_interp_prim /prim_evals_to; naive_solver.
   Qed.
 
   Lemma sP_Bool_I Γ b: ⊢ Γ s⊨p pv (vbool b): oBool, 0.
   Proof.
-    iIntros "!> * _ /=";
+    iIntros "%ρ _ /=";
       rewrite path_wp_pv_eq /= /pure_interp_prim /prim_evals_to; naive_solver.
   Qed.
 
@@ -73,7 +73,7 @@ Section Sec.
     Γ s⊨ e1 : oPrim B1 -∗
     Γ s⊨ tun u e1 : oPrim Br.
   Proof.
-    iIntros "#He1 !> %ρ #Hg !>".
+    iIntros "#He1 %ρ #Hg".
     smart_wp_bind (UnCtx _) v1 "%Ha1" ("He1" with "Hg"); iClear "He1 Hg".
     by iApply wp_wand; [iApply wp_un|iIntros (? [??])].
   Qed.
@@ -98,7 +98,7 @@ Section Sec.
     Γ s⊨ e2 : oPrim B2 -∗
     Γ s⊨ tbin b e1 e2 : oPrim Br.
   Proof.
-    iIntros "#He1 #He2 !> /= %ρ #Hg !>". rewrite /oPrim/= /pure_interp_prim.
+    iIntros "#He1 #He2 /= %ρ #Hg". rewrite /oPrim/= /pure_interp_prim.
     smart_wp_bind (BinLCtx _ _) v1 "%Ha1" ("He1" with "Hg"); iClear "He1".
     smart_wp_bind (BinRCtx _ _) v2 "%Ha2" ("He2" with "Hg"); iClear "He2"; ev.
     by iApply wp_wand; [iApply wp_bin|iIntros (? [??])].
@@ -120,7 +120,7 @@ Section Sec.
     Γ s⊨ e : oBool -∗ Γ s⊨ e1 : T -∗ Γ s⊨ e2 : T -∗
     Γ s⊨ tif e e1 e2 : T.
   Proof.
-    iIntros "#He #He1 #He2 !> /= %ρ #Hg !>".
+    iIntros "#He #He1 #He2 /= %ρ #Hg".
     smart_wp_bind (IfCtx _ _) v "#Ha" ("He" with "[]").
     rewrite /pure_interp_prim/=; iDestruct "Ha" as %([] & ->);
       (rewrite -wp_pure_step_later; last done);
