theories/Dot/semtyp_lemmas/tproj_lr.v
@@ -48,7 +48,7 @@ Section existentials.
     oLaterN i (oShift S) :: Γ s⊨ T <:[i] oShift U -∗
     Γ s⊨ oExists S T <:[i] U.
   Proof.
-    rewrite !sstpd_to_sstpi; iIntros "/= #Hstp !> %ρ %v Hg".
+    rewrite !sstpd_to_sstpi; iIntros "/= #Hstp %ρ %v Hg".
     iDestruct 1 as (w) "[HS HT]".
     iApply ("Hstp" $! (w .: ρ) v with "[$Hg $HS] HT").
   Qed.
@@ -59,7 +59,7 @@ Section existentials.
     Γ s⊨ T <:[i] opSubst p U -∗
     Γ s⊨ T <:[i] oExists S U.
   Proof.
-    iIntros "/= #HpS #Hstp !> %ρ #Hg".
+    iIntros "/= #HpS #Hstp %ρ #Hg".
     iSpecialize ("HpS" with "Hg"); iSpecialize ("Hstp" with "Hg"); iNext i.
     iApply (subtype_trans with "Hstp"); iIntros "%v HvUp".
     iDestruct (path_wp_agree with "HpS HvUp") as (w _) "?".
@@ -101,7 +101,7 @@ Section type_proj_setoid_equality.
 
   Lemma oProjN_eq_2 n A T args ρ v :
     oProjN n A T args ρ v ⊣⊢
-    ∃ w d ψ, ⌜w @ A ↘ d⌝ ∧ oClose T ρ w ∧ d ↗n[ n ] ψ ∧ ▷ □ ψ args v.
+    ∃ w d ψ, ⌜w @ A ↘ d⌝ ∧ oClose T ρ w ∧ d ↗n[ n ] ψ ∧ ▷ ψ args v.
   Proof.
     rewrite oProjN_eq; f_equiv => w.
     rewrite and_exist_l; f_equiv => ψ; rewrite and_exist_l; f_equiv => d.
@@ -163,7 +163,7 @@ Section type_proj.
     Γ s⊨ T <:[i] U -∗
     Γ s⊨ oProj A T <:[i] oProj A U.
   Proof.
-    iIntros "#Hsub !> %ρ Hg %v"; iSpecialize ("Hsub" with "Hg"); iNext i.
+    iIntros "#Hsub %ρ Hg %v"; iSpecialize ("Hsub" with "Hg"); iNext i.
     (**
       From [T <: U] we must show [T#A <: U#A], that is, that any [v] in [T#A]
       is in [U#A]. Recall the definition of [T#A]:
@@ -188,7 +188,7 @@ Section type_proj.
   Lemma sProj_Stp_U A Γ L U i :
     ⊢ Γ s⊨ oProj A (cTMem A L U) <:[i] U.
   Proof.
-    iIntros "!> %ρ Hg %v"; iNext i.
+    iIntros "%ρ Hg %v"; iNext i.
     rewrite oProjN_eq; iDestruct 1 as (w) "(HTw & HselV)".
     (*
       After unfolding definitions, we must show that [v] is in [U],
